ap/util.lean
@@ -1,0 +1,18 @@
+import tactic.induction
+import data.int.basic
+import data.set.basic
+import data.list
+
+noncomputable theory
+open_locale classical
+
+lemma snoc_eq_snoc_iff {α : Type*} {xs ys : list α} {x y : α} :
+  xs ++ [x] = ys ++ [y] ↔ xs = ys ∧ x = y :=
+begin
+  split; intro h,
+  { rw list.append_eq_append_iff at h, cases h; rcases h with ⟨zs, h₁, h₂⟩;
+    { have h₃ := congr_arg list.length h₂, simp at h₃,
+      rw list.length_eq_zero at h₃, cases h₃, simp at h₁ h₂,
+      exact ⟨h₁.symm, h₂⟩ <|> exact ⟨h₁, h₂.symm⟩ }},
+  { rw [h.1, h.2] },
+end
